CoqCode/Automations.v
@@ -1,0 +1,16 @@
+Require Import Metalib.Metatheory.
+Require Import Coq.Program.Equality.
+Require Import Language Subtyping Auxiliaries Notations.
+
+Lemma trm_top_checked_by_toplike :
+  forall (A : typ),
+    toplike A ->
+    typing nil nil check_mode trm_top A.
+Proof.
+  intros.
+  eapply typing_sub; eauto.
+  eapply toplike_sub_top. assumption.
+Qed.
+
+Hint Resolve trm_top_checked_by_toplike : core.
+    
