CoqCode/Deterministic.v
@@ -1,11 +1,11 @@
 Require Import Coq.Program.Equality.
-Require Import Language Notations Auxiliaries Subtyping.
+Require Import Language Notations Auxiliaries Subtyping Automations.
 Require Import Strings.String.
 
 Set Printing Parentheses.
 
 Lemma tred_ord_toplike : forall (e e' : trm) (A : typ),
-    ordinary A -> toplike A -> typedred e A e' -> e' = (trm_anno trm_top typ_top).
+    ordinary A -> toplike A -> typedred e A e' -> e' = (trm_anno trm_top A).
 Proof.
   intros e e' A H_ord H_top H_tred.
   dependent induction H_tred; subst; eauto.
@@ -16,7 +16,8 @@ Qed.
 
 Lemma tred_toplike :
   forall (A : typ),
-    toplike A -> forall e1 e2 e1' e2' : trm, typedred e1 A e1' -> typedred e2 A e2' -> e1' = e2'.
+    toplike A ->
+    forall e1 e2 e1' e2' : trm, typedred e1 A e1' -> typedred e2 A e2' -> e1' = e2'.
 Proof.
   intros A Htop.
   dependent induction Htop; intros e1 e2 e1' e2' H_tred1 H_tred2.
@@ -62,7 +63,8 @@ Proof.
     inversion Hval; subst; clear Hval.
     inversion Htyp; subst; clear Htyp.
     inversion H7; subst; clear H7.
-    eapply sub_arrow; eauto 3.
+    + eapply sub_arrow; eauto 3.
+    (* + dependent destruction H2. eapply toplike_sub_toplike in H2; eauto. contradiction. *)
   - intros B0 Htyp.
     inversion Hval; subst; clear Hval.
     inversion Htyp; subst; clear Htyp.
@@ -208,7 +210,6 @@ Proof.
     + inversion Hred2; subst; clear Hred2; eauto.
 Qed.
 
-
 Lemma tred_consistency :
   forall (v v1 v2 : trm) (A B C : typ),
     value v -> typing nil nil infer_mode v C ->
@@ -236,16 +237,15 @@ Proof.
   intros v v' A Hval Htyp Hred.
   induction Hred.
   - exists typ_int. constructor; eauto 3.
-  - exists typ_top. constructor; eauto 3.
+  - exists A. eapply typing_anno; eauto.
   - destruct Htyp.
     inversion H2; subst.
     inversion H7; subst.
-    exists (typ_arrow C D).
-    eapply typing_anno; eauto 3.
-    (* so we need checked subsumption here *)
-    assert (Hsub: sub (typ_arrow A B) (typ_arrow C D)).
-    apply sub_arrow. assumption. assumption.
-    eapply typing_sub_check. apply H8. apply Hsub.
+    + exists (typ_arrow C D).
+      eapply typing_anno; eauto 3.
+      assert (Hsub: sub (typ_arrow A B) (typ_arrow C D)).
+      apply sub_arrow. assumption. assumption.
+      eapply typing_sub_check. apply H8. apply Hsub.
   - apply IHHred. inversion Hval; subst. assumption.
     destruct Htyp. inversion H0; subst.
     + exists A0. assumption.
@@ -311,14 +311,15 @@ Proof.
   intros A B1 B2 S Has1 Has2.
   generalize dependent B2.
   dependent induction Has1; intros.
-  - dependent destruction Has2. reflexivity.
   - dependent destruction Has2.
-    assert (Heq: D = D0).
-    eapply IHHas1; eauto.
-    rewrite Heq; eauto.
+    + reflexivity.
+  - dependent destruction Has2.
+    + assert (Heq: D = D0).
+      eapply IHHas1; eauto.
+      rewrite Heq. reflexivity.
   - dependent destruction Has2.
     + eapply IHHas1; eauto.
-    + destruct H0. admit.
+    + admit. 
   - dependent destruction Has2.
     + admit.
     + eapply IHHas1; eauto.
@@ -335,24 +336,23 @@ Admitted.
 
 (* some inversion lemmas may help since premises are a lot *)
 Lemma papp_determinism :
-  forall (r vl e1 e2 : trm),
-    rvalue r -> value vl ->
+  forall (v vl e1 e2 : trm),
+    value v -> value vl ->
     (exists (B : typ), typing nil nil infer_mode vl B) ->
-    papp r vl e1 -> papp r vl e2 -> e1 = e2.
+    papp v vl e1 -> papp v vl e2 -> e1 = e2.
 Proof.
-  intros r vl e1 e2 Hrv Hv Htyp Hp1 Hp2.
+  intros v vl e1 e2 Hrv Hv Htyp Hp1 Hp2.
   generalize dependent e2.
   dependent induction Hp1.
   - intros. inversion Hp2; subst.
     + reflexivity.
     + dependent destruction H. contradiction.
-  - intros. inversion Hp2; subst. reflexivity.
   - intros. dependent destruction Hp2.
     + dependent destruction H1. contradiction.
     + assert (v' = v'0). eapply tred_determinism; eauto.
       rewrite H3; eauto.
   - intros. apply IHHp1; eauto.
-    + dependent destruction Hrv. dependent destruction H. apply rvalue_v. auto.
+    + dependent destruction Hrv. assumption.
     + dependent destruction Hp2.
       * apply Hp2.
       * (* try to invert this case *)
@@ -365,13 +365,13 @@ Proof.
         assert (A0 = A2). eapply ptype_determinsm. apply H. apply H9.
         assert (A0 = B2). eapply ptype_determinsm; eauto.
         assert (A2 = B2). rewrite <- H7. rewrite <- H8. reflexivity. subst. rename B2 into C.
-        dependent destruction Hrv. dependent destruction H.
+        dependent destruction Hrv.
         assert (v1 = v2). eapply ptype_merge_same; eauto. subst. eauto.
         (* we need a lemma inversion of two brach of appsub *)
         (* well, that's basically determinsm of appsub *)
         (* try to find a contradiction: disjoint? in ptype? *)
   - intros. apply IHHp1; eauto.
-    + dependent destruction Hrv. dependent destruction H. apply rvalue_v. eauto.
+    + dependent destruction Hrv. assumption.
     + dependent destruction Hp2.
       * inversion H1; subst.
         inversion H5; subst.
@@ -382,7 +382,7 @@ Proof.
         assert (A0 = A2). eapply ptype_determinsm; eauto.
         assert (A0 = B2). eapply ptype_determinsm. apply H. apply H11.
         assert (A2 = B2). rewrite <- H7. rewrite <- H8. reflexivity. subst. rename B2 into C.
-        dependent destruction Hrv. dependent destruction H.
+        dependent destruction Hrv.
         assert (v1 = v2). eapply ptype_merge_same; eauto. subst. eauto.
       * apply Hp2.
 Qed.
@@ -431,25 +431,13 @@ Proof.
       * apply H2. constructor. constructor.
     + intros. unfold not. intros.
       inversion H; subst; clear H.
-      Focus 2.
-      * apply H2. constructor. constructor.
       * inversion H2.
-Qed.
-
-Lemma rvalue_cannot_step_further :
-  forall (r : trm),
-    rvalue r -> forall (e : trm), not (step r e).
-Proof.
-  intros r Hr.
-  induction Hr.
-  - eapply value_cannot_step_further. assumption.
-  - intros. unfold not. intros.
-    inversion H.
+      * apply H2. constructor. constructor.
 Qed.
 
 Lemma app_check_inversion :
-  forall (r vl : trm) (A : typ),
-    rvalue r -> value vl -> typing nil nil check_mode (trm_app r vl) A ->
+  forall (v vl : trm) (A : typ),
+    value v -> value vl -> typing nil nil check_mode (trm_app v vl) A ->
     exists (B : typ), typing nil nil infer_mode vl B.
 Proof.
   intros r vl A Hrv Hv Hchk.
@@ -505,8 +493,8 @@ Proof.
     reflexivity.
   - intros A Htyp e2 Hred2.
     inversion Hred2; subst. (* papp and 2 congruence rules *)
-    + eapply app_check_inversion in Htyp; eauto. eapply papp_determinism; eauto.
-    + eapply rvalue_cannot_step_further in H5. inversion H5. auto.
+    + eapply app_check_inversion in Htyp; eauto. apply papp_determinism with (v:=v) (vl:=vl); eauto.
+    + eapply value_cannot_step_further in H5. inversion H5. auto.
     + eapply value_cannot_step_further in H6. inversion H6. auto.
   - intros A0 Htyp e2 Hred2.
     dependent destruction Hred2.
@@ -524,7 +512,7 @@ Proof.
       * rewrite Heq. reflexivity.
   - intros A Htyp e0 Hred2.
     dependent destruction Hred2.
-    + eapply rvalue_cannot_step_further in Hred1; eauto. contradiction.
+    + eapply value_cannot_step_further in Hred1; eauto. contradiction.
     + assert (Heq: e1' = e1'0).
       dependent destruction Htyp.
       * eapply IHHred1; eauto.
@@ -541,11 +529,11 @@ Proof.
         (* dependent destruction Hred1. dependent destruction Hred2. *)
         (* eapply tred_determinism; eauto. *)
       * rewrite Heq; eauto.
-    + eapply rvalue_cannot_step_further in Hred1. contradiction. assumption.
+    + eapply value_cannot_step_further in Hred1. contradiction. assumption.
   - intros A Htyp e0 Hred2.
     dependent destruction Hred2.
     + eapply value_cannot_step_further in Hred1. contradiction. assumption.
-    + eapply rvalue_cannot_step_further in Hred2. contradiction. assumption.
+    + eapply value_cannot_step_further in Hred2. contradiction. assumption.
     + assert (Heq: e2' = e2'0).
       dependent destruction Htyp.
       * eapply IHHred1; eauto.
