CoqCode/Soundness.v
@@ -1,6 +1,29 @@
 Require Import Metalib.Metatheory.
 Require Import Coq.Program.Equality.
-Require Import Language Subtyping Auxiliaries Notations Deterministic.
+Require Import Language Subtyping Auxiliaries Notations Deterministic Automations.
+
+Lemma typing_check_merge_distro :
+  forall (v : trm) (A B : typ),
+    typing nil nil check_mode v (typ_and A B) ->
+    (typing nil nil check_mode v A) /\ (typing nil nil check_mode v B).
+Proof.
+  intros. split.
+  - eapply typing_sub_check.
+    eapply H. apply sub_and_l. eapply sub_reflexivity.
+  - eapply typing_sub_check.
+    eapply H. apply sub_and_r. eapply sub_reflexivity.
+Qed.
+
+Lemma sub_type_and_distro :
+  forall (A B C : typ),
+    ordinary C ->
+    sub (typ_and A B) C ->
+    sub A C \/ sub B C.
+Proof.
+  intros.
+  dependent induction H0; eauto.
+  inversion H.
+Qed.
 
 Theorem tred_preservation :
   forall (v v' : trm) (A: typ),
@@ -12,7 +35,7 @@ Proof.
   intros v v' A Hv Htyp Hred.
   dependent induction Hred.
   - eapply typing_anno; eauto.
-  - admit. (* appsub and toplike *)
+  - eapply typing_anno; eauto.
   - apply typing_anno; eauto.
     dependent destruction Htyp.
     dependent destruction Htyp.
@@ -23,65 +46,82 @@ Proof.
     + apply IHHred; eauto.
       eapply typing_sub.
       eapply Htyp1.
-      admit.
+      eapply tred_sub. apply Hv1. apply Hred. apply Htyp1.
     + apply IHHred; eauto.
       eapply typing_sub.
       eapply Htyp1.
-      admit.
+      eapply tred_sub. apply Hv1. apply Hred. apply Htyp1.
   - dependent destruction Hv.
     dependent destruction Htyp.
     dependent destruction Htyp.
     + apply IHHred; eauto.
       eapply typing_sub.
       apply Htyp2.
-      admit.
+      eapply tred_sub. apply Hv2. apply Hred. apply Htyp2.
     + apply IHHred; eauto.
       eapply typing_sub.
       apply Htyp2.
-      admit.
+      eapply tred_sub. apply Hv2. apply Hred. apply Htyp2.
   - eapply typing_merge_value.
     + eapply tred_value; eauto.
     + eapply tred_value; eauto.
     + eapply IHHred1. assumption.
-      admit.
+      eapply typing_check_merge_distro in Htyp. destruct Htyp.
+      assumption.
     + eapply IHHred2. assumption.
-      admit.
-    + eapply tred_consistency; eauto.
-Admitted.
+      eapply typing_check_merge_distro in Htyp. destruct Htyp.
+      assumption.
+    + dependent destruction Htyp.
+      * inversion Hv.
+      * eapply tred_consistency; eauto.
+Qed.
 
-Lemma papp_preservation :
-  forall (r v e : trm) (A B : typ) (S : arg),
-    rvalue r -> value v ->
-    papp r v e ->
-    typing nil nil infer_mode v A ->
-    typing nil (cons A S) infer_mode r (typ_arrow A B) ->
+Lemma papp_preservation_infer:
+  forall (v vl e : trm) (A B : typ) (S : arg),
+    value v -> value vl ->
+    papp v vl e ->
+    typing nil nil infer_mode vl A ->
+    typing nil (cons A S) infer_mode v (typ_arrow A B) ->
     typing nil S infer_mode e B.
 Proof.
-  intros r v e A B Hr Hv Hp Htyp1 Htyp2.
-  generalize dependent A.
-  generalize dependent B.
-  dependent induction Hp; intros.
-Admitted.
+  Admitted.
 
-Lemma papp_preservation_dir :
-  forall (r v e : trm) (A B : typ) (S : arg) (dir : mode),
-    rvalue r -> value v ->
-    papp r v e ->
-    typing nil nil infer_mode v A ->
-    typing nil (cons A S) dir r (typ_arrow A B) ->
+(* this lemma may be generalized wrongly *)
+Lemma papp_preservation :
+  forall (v vl e : trm) (A B : typ) (S : arg) (dir : mode),
+    value v -> value vl ->
+    papp v vl e ->
+    typing nil nil infer_mode vl A ->
+    typing nil (cons A S) dir v (typ_arrow A B) ->
     typing nil S dir e B.
 Proof.
-  intros. 
+  intros v vl e A B S dir Hr Hv Hp Htyp1 Htyp2.
+  generalize dependent A.
+  dependent induction Hp; intros.
+  - dependent destruction Htyp2. 
 Admitted.
   
 Lemma papp_preservation_check :
-  forall (r v e : trm) (A B : typ),
-    rvalue r -> value v ->
-    papp r v e ->
-    typing nil nil infer_mode v A ->
-    typing nil nil check_mode r (typ_arrow A B) ->
+  forall (v vl e : trm) (A B : typ),
+    value v -> value vl ->
+    papp v vl e ->
+    typing nil nil check_mode v (typ_arrow A B) ->
+    typing nil nil infer_mode vl A ->
     typing nil nil check_mode e B.
 Proof.
+  intros v vl e A B Hv Hvl Hp Htyp1 Htyp2.
+  dependent induction Htyp1.
+Admitted.
+
+Lemma appsub_typing :
+  forall (e : trm) (A B : typ) (S : arg),
+    typing nil nil infer_mode e A ->
+    appsub S A B ->
+    typing nil S infer_mode e B.
+Proof.
+  intros e A B S Htyp Has.
+  generalize dependent  e.
+  dependent induction Has; intros; eauto.
 Admitted.
 
 Theorem preservation :
@@ -103,15 +143,15 @@ Proof.
   - dependent destruction Hred.
     + assert (Htyp2: typing nil nil infer_mode v' A).
       eapply tred_preservation; eauto.
-      admit. (* Htyp2, H *)
+      eapply appsub_typing; eauto.
     + eapply typing_anno. assumption.
       eapply IHHtyp; eauto.
   - dependent destruction Hred.
-    + eapply papp_preservation; eauto.
+    + eapply papp_preservation_infer with (v:=e1) (vl:=e2); eauto.
     + eapply typing_app1; eauto.
     + eapply typing_app1; eauto.
   - dependent destruction Hred.
-    + eapply papp_preservation_check; eauto.
+    + eapply papp_preservation_check with (v:=e1) (vl:=e2); eauto.
     + eapply typing_app2; eauto.
     + eapply typing_app2; eauto.
   - assert (Htyp2: typing nil nil infer_mode e' B).
@@ -127,14 +167,9 @@ Proof.
   - assert (Htyp2: typing nil S infer_mode e' B).
     eapply IHHtyp; eauto.
     dependent destruction Hred.
-    + admit.
-    + 
-    (*
-      The problem is
-      reduction of merge picking appears at papp
-      typing of merge picking appears at merge
-     *)
-Admitted.
+    + eapply typing_merge_pick; eauto.
+    + eapply typing_merge_pick; eauto.
+Qed.
 
 Theorem tred_progress :
   forall (v : trm) (A : typ),
@@ -142,7 +177,9 @@ Theorem tred_progress :
     exists v', typedred v A v'.
 Proof.
   intros v A Hv Htyp.
-Admitted.
+  dependent induction A.
+  - dependent destruction Htyp; try solve [inversion Hv].
+Admitted.    
 
 Lemma pvalue_cannot_be_value :
   forall (e : trm),
@@ -180,18 +217,18 @@ Proof.
 Qed.
 
 Theorem progress :
-  forall (e : trm) (dir : mode) (A : typ) (S : arg),
+  forall (e : trm) (A : typ) (S : arg) (dir : mode),
     typing nil S dir e A ->
     value e \/ exists e', step e e'.
 Proof.
-  intros e dir A S Htyp.
+  intros e A S dir Htyp.
   dependent induction Htyp.
   - right. exists (trm_anno (trm_nat n) typ_int).
     apply step_int_anno.
   - right. exists (trm_anno trm_top typ_top).
     apply step_top_anno.
   - inversion H0.
-  - left. constructor; eauto.
+  - left. constructor. constructor.
   - destruct IHHtyp; eauto.
     + right. assert (Hv: value e); eauto.
       eapply tred_progress in H0; eauto.
@@ -202,8 +239,8 @@ Proof.
       destruct Hval.
       * left. assumption.
       * right. exists (trm_anno x A). eapply step_anno. assumption. assumption.
-  - right. destruct IHHtyp1; destruct IHHtyp2; eauto.
-    + admit. (* the diff from snow's is her system has a arrTyp relation ? *)
+  - destruct IHHtyp1; destruct IHHtyp2; eauto.
+    + right. admit.
     + admit.
     + admit.
     + admit.
@@ -212,3 +249,19 @@ Proof.
   - destruct IHHtyp1; destruct IHHtyp2; eauto.
 Admitted.
 (* the typing merge has some problems with reduction *)
+
+Theorem progress_infer :
+  forall (e : trm) (A : typ) (S : arg),
+    typing nil S infer_mode e A ->
+    value e \/ exists e', step e e'.
+Proof.
+  intros e A S Htyp.
+  dependent induction Htyp.
+  - right. exists (trm_anno (trm_nat n) typ_int).
+    apply step_int_anno.
+  - right. exists (trm_anno trm_top typ_top).
+    apply step_top_anno.
+  - inversion H0.
+  -
+Admitted.
+    
